continue work on new formalisation of graphs & clique

theories/L/Complexity/Problems/FlatUGraph.v
@@ -3,6 +3,7 @@ From Undecidability.L.Tactics Require Import LTactics GenEncode.
 From Undecidability.L.Datatypes Require Import LLists LLNat LProd.
 From PslBase Require Import FinTypes. 
 From Undecidability.L.Complexity.Problems Require Import UGraph.
+From Undecidability.L.Complexity.Cook Require Import FlatFinTypes.
 
 (** *Flat representation of an undirected graph. *)
 
@@ -21,32 +22,78 @@ Definition fedges_wf n (E : list fedge) := forall e, e el E -> fedge_wf n e.
 Definition fgraph_wf G := match G with (V, E) => fedges_symmetric E /\ fedges_wf V E end. 
 
 Definition fedge_eqb := prod_eqb Nat.eqb Nat.eqb.
-Definition ledges_edge_in_decb E e := list_in_decb fedge_eqb E e. 
-Definition lgraph_edge_in_decb G e := match G with (V, E) => ledges_edge_in_decb E e end. 
+Definition fedges_edge_in_decb E e := list_in_decb fedge_eqb E e. 
+Definition fgraph_edge_in_decb G e := match G with (V, E) => fedges_edge_in_decb E e end. 
 
+Definition isfVertex (V : fvertex) (v : fvertex) := v < V.
 
 (** Boolean deciders for some of the above definitions*)
 Definition fedges_symmetric_decb (E : list fedge) := 
-  forallb (fun e => let (v1, v2) := e in ledges_edge_in_decb E (v2, v1)) E. 
+  forallb (fun e => let (v1, v2) := e in fedges_edge_in_decb E (v2, v1)) E. 
 
 Definition fedge_wf_decb n e := let (v1, v2) := e in Nat.ltb v1 n && Nat.ltb v2 n. 
 Definition fedges_wf_decb n E := forallb (fedge_wf_decb n) E.
 
-Definition fraph_wf_decb G := let (V, E) := G in fedges_symmetric_decb E && fedges_wf_decb V E. 
+Definition fgraph_wf_decb G := let (V, E) := G in fedges_symmetric_decb E && fedges_wf_decb V E. 
 
-(*Lemma fedge_eqb_iff e1 e2 : fedge_eqb e1 e2 = true <-> e1 = e2. *)
+Definition isfVertex_decb V v := Nat.ltb v V. 
 
+Proposition fedge_eqb_spec e1 e2 : reflect (e1 = e2) (fedge_eqb e1 e2).
+Proof. 
+  unfold fedge_eqb. apply prod_eqb_spec; apply Nat.eqb_spec.  
+Qed.
+
+Corollary fedge_eqb_iff e1 e2 : e1 = e2 <-> fedge_eqb e1 e2 = true.
+Proof.
+  apply reflect_iff, fedge_eqb_spec. 
+Qed. 
+
+Proposition fedges_edge_in_decb_iff E e: fedges_edge_in_decb E e = true <-> e el E. 
+Proof. 
+  apply list_in_decb_iff, fedge_eqb_iff.
+Qed. 
+
+Proposition fedge_wf_decb_iff n e : fedge_wf_decb n e = true <-> fedge_wf n e. 
+Proof. 
+  unfold fedge_wf_decb, fedge_wf. destruct e. 
+  rewrite andb_true_iff, !Nat.ltb_lt. easy.
+Qed. 
+
+Proposition fedges_symmetric_decb_iff E : fedges_symmetric_decb E = true <-> fedges_symmetric E. 
+Proof. 
+  unfold fedges_symmetric_decb, fedges_symmetric. 
+  rewrite forallb_forall. split; intros H. 
+  - intros v1 v2 H1. apply fedges_edge_in_decb_iff, (H (v1, v2)), H1. 
+  - intros [v1 v2] H1. apply fedges_edge_in_decb_iff, H, H1. 
+Qed. 
+
+Proposition fedges_wf_decb_iff n E : fedges_wf_decb n E = true <-> fedges_wf n E. 
+Proof. 
+  unfold fedges_wf_decb, fedges_wf. rewrite forallb_forall. setoid_rewrite fedge_wf_decb_iff. easy.
+Qed.
+
+Proposition fgraph_wf_decb_iff G : fgraph_wf_decb G = true <-> fgraph_wf G. 
+Proof. 
+  unfold fgraph_wf_decb, fgraph_wf. 
+  destruct G. rewrite andb_true_iff, fedges_symmetric_decb_iff, fedges_wf_decb_iff. 
+  easy.
+Qed. 
+
+Proposition isfVertex_decb_iff V v : isfVertex_decb V v = true <-> isfVertex V v. 
+Proof. 
+  unfold isfVertex_decb, isfVertex. apply Nat.ltb_lt.
+Qed.
 
 (** We relate UGraph and fgraph instances in the following way *)
-Definition isFlatVerticesOf V (finV : finType) := V = |elem finV|.
+Definition isFlatVerticesOf V (finV : finType) := finRepr finV V.
+Definition isFlatVertexOf (finV : finType) V (v : finV):= finReprEl' V v. 
 
-Definition isFlatVertexOf (finV : finType) V (v : finV):= V = index v. 
-
-Inductive isFlatEdgesOf E V (finV : finType) (finE : finV -> finV -> Prop) : Prop := 
+Inductive isFlatEdgesOf E V (finV : finType) (finE : finV * finV -> Prop) : Prop := 
   mkIsFlatEdgesOf 
-    (R__flatVertices : isFlatVerticesOf V finV)
     (R__edgesSound : forall v1 v2, (v1, v2) el E -> fedge_wf V (v1, v2) /\ 
-                                                    exists (V1 V2 : finV), finE V1 V2 /\ isFlatVertexOf v1 V1 /\ isFlatVertexOf v2 V2)
-    (R__edgesComplete : forall (v1 v2 : finV), finE v1 v2 -> (index v1, index v2) el E)
+                                                    exists (V1 V2 : finV), finE (V1, V2) /\ isFlatVertexOf v1 V1 /\ isFlatVertexOf v2 V2)
+    (R__edgesComplete : forall (v1 v2 : finV), finE (v1, v2) -> (index v1, index v2) el E)
     : isFlatEdgesOf E V finE.
                                                   
+Definition isFlatGraphOf (g : fgraph) (UG : UGraph) := 
+  let (fV, fE) := g in isFlatVerticesOf fV (V UG) /\ isFlatEdgesOf fE fV (@E UG). 
