theories/L/Datatypes/LLNat.v
@@ -2,10 +2,11 @@ From Undecidability.L.Tactics Require Export LTactics GenEncode.
 Require Import PslBase.Numbers.
 
 Require Import Nat Undecidability.L.Datatypes.LBool Undecidability.L.Datatypes.LProd.
+Require Undecidability.L.Datatypes.LNat. 
 (** ** Encoding of natural numbers *)
 
-Run TemplateProgram (tmGenEncode "nat_enc" nat).
-Hint Resolve nat_enc_correct : Lrewrite.
+(*Run TemplateProgram (tmGenEncode "nat_enc" nat).*)
+(*Hint Resolve nat_enc_correct : Lrewrite.*)
 
 Instance termT_S : computableTime' S (fun _ _ => (1,tt)).
 Proof.
@@ -65,13 +66,23 @@ Proof.
   solverec. all: unfold nat_eqb_time, c__nat_eqb, c__nat_eqb2; solverec. 
 Defined.
 
-Instance termT_nat_min : computableTime' Nat.min (fun x _ => (5, fun y _ => (8 + 15 * min x y, tt))).
+Definition c__min1 := 5.
+Definition c__min2 := 15. 
+Definition min_time x y := (min x y + 1) * c__min2. 
+Instance termT_nat_min : computableTime' Nat.min (fun x _ => (c__min1, fun y _ => (min_time x y, tt))).
 Proof. 
   extract. solverec. 
-Qed. 
+  all: unfold min_time, c__min1, c__min2; solverec. 
+Defined. 
 
-Instance termT_nat_max : computableTime' Nat.max (fun x _ => (5, fun y _ => (8 + 15 * min x y, tt))).
-Proof. extract. solverec. Qed. 
+Definition c__max1 := 5.
+Definition c__max2 := 15. 
+Definition max_time x y := (min x y + 1) * c__max2. 
+Instance termT_nat_max : computableTime' Nat.max (fun x _ => (c__max1, fun y _ => (max_time x y, tt))).
+Proof. 
+  extract. solverec. 
+  all: unfold max_time, c__max1, c__max2; solverec. 
+Defined. 
 
 Definition c__pow1 := 5.
 Definition c__pow2 := 10 + c__mult1.
@@ -106,36 +117,36 @@ Defined.
 
 (* now some more encoding-related properties:*)
 
-Fixpoint nat_unenc (s : term) :=
-  match s with
-  | lam (lam #1) => Some 0
-  | lam (lam (app #0 s)) => match nat_unenc s with Some n => Some (S n) | x=>x end
-  | _ => None
-  end.
+(*Fixpoint nat_unenc (s : term) :=*)
+  (*match s with*)
+  (*| lam (lam #1) => Some 0*)
+  (*| lam (lam (app #0 s)) => match nat_unenc s with Some n => Some (S n) | x=>x end*)
+  (*| _ => None*)
+  (*end.*)
 
-Lemma unenc_correct m : (nat_unenc (nat_enc m)) = Some m.
-Proof.
-  induction m; simpl; now try rewrite IHm.
-Qed.
+(*Lemma unenc_correct m : (nat_unenc (LNat.nat_enc m)) = Some m.*)
+(*Proof.*)
+  (*induction m; simpl; now try rewrite IHm.*)
+(*Qed.*)
 
-Lemma unenc_correct2 t n : nat_unenc t = Some n -> nat_enc n = t.
-Proof with try solve [Coq.Init.Tactics.easy].
-  revert n. eapply (size_induction (f := size) (p := (fun t => forall n, nat_unenc t = Some n -> nat_enc n = t))). clear t. intros t IHt n H.
-  destruct t. easy. easy.
-  destruct t. easy. easy.
-  destruct t. 3:easy.
-  -destruct n0. easy. destruct n0. 2:easy. inv H. easy.
-  -destruct t1. 2-3:easy. destruct n0. 2:easy. simpl in H. destruct (nat_unenc t2) eqn:A.
-   +apply IHt in A;simpl;try omega. destruct n. inv H. simpl. congruence.
-   +congruence.
-Qed.
+(*Lemma unenc_correct2 t n : nat_unenc t = Some n -> LNat.nat_enc n = t.*)
+(*Proof with try solve [Coq.Init.Tactics.easy].*)
+  (*revert n. eapply (size_induction (f := size) (p := (fun t => forall n, nat_unenc t = Some n -> nat_enc n = t))). clear t. intros t IHt n H.*)
+  (*destruct t. easy. easy.*)
+  (*destruct t. easy. easy.*)
+  (*destruct t. 3:easy.*)
+  (*-destruct n0. easy. destruct n0. 2:easy. inv H. easy.*)
+  (*-destruct t1. 2-3:easy. destruct n0. 2:easy. simpl in H. destruct (nat_unenc t2) eqn:A.*)
+   (*+apply IHt in A;simpl;try omega. destruct n. inv H. simpl. congruence.*)
+   (*+congruence.*)
+(*Qed.*)
 
-Lemma dec_enc t : dec (exists n, t = nat_enc n).
-Proof.
-  destruct (nat_unenc t) eqn:H.
-  - left. exists n. now eapply unenc_correct2 in H.
-  - right. intros [n A]. rewrite A in H. rewrite unenc_correct in H. inv H.
-Qed.
+(*Lemma dec_enc t : dec (exists n, t = nat_enc n).*)
+(*Proof.*)
+  (*destruct (nat_unenc t) eqn:H.*)
+  (*- left. exists n. now eapply unenc_correct2 in H.*)
+  (*- right. intros [n A]. rewrite A in H. rewrite unenc_correct in H. inv H.*)
+(*Qed.*)
 
 Definition c__natsizeO := 4.
 Definition c__natsizeS := 4.
@@ -143,13 +154,13 @@ Lemma size_nat_enc (n:nat) :
   size (enc n) = n * c__natsizeS + c__natsizeO.
 Proof.
   unfold c__natsizeS, c__natsizeO. 
-  induction n;cbv [enc registered_nat_enc] in *. all:cbn [size nat_enc] in *. all:solverec.
+  induction n;cbv [enc LNat.registered_nat_enc] in *. all:cbn [size LNat.nat_enc] in *. all:solverec.
 Qed.
 
 Lemma size_nat_enc_r (n:nat) :
   n <= size (enc n).
 Proof.
-    induction n;cbv [enc registered_nat_enc] in *. all:cbn [size nat_enc] in *. all:solverec.
+    induction n;cbv [enc LNat.registered_nat_enc] in *. all:cbn [size LNat.nat_enc] in *. all:solverec.
 Qed.
 
 
